ECCA/typing_lemmas.v
@@ -18,69 +18,101 @@ induction pT; names; eauto; intros.
   names. specialize IHpT2 with (r:=(r,,x)%ren). apply IHpT2. apply ctx_rename. auto.
 Qed.
 
-Definition Type_weakening Γ e A (pT: (Γ ⊢ e : A)):=
+(* vvv Not true vvv*)
+(* Definition WellFormed_weakening Γ (pWF: (⊢ Γ)):=
   forall r Δ,
     Γ =[r]=> Δ ->
+    (⊢ Δ). *)
+
+Lemma Types_only_if_wellformed Γ e A:
+(Γ ⊢ e : A)->
+(⊢ Γ). 
+Proof.
+intros.
+induction H; auto.
+Qed.
+Hint Resolve Types_only_if_wellformed.
+
+Lemma Type_weakening Γ e A (pT: (Γ ⊢ e : A)):
+  forall r Δ,
+    Γ =[r]=> Δ ->
+    (⊢ Δ) ->
     (Δ ⊢ ([r] e) : [r] A).
+Proof. 
+induction pT; auto.
+all: try (intros; constructor; eauto; fail).
++ intros. names. destruct H1 eqn:H3. 
+  rewrite applyt_is_applyv with (rn:=total). names. apply aT_Var.
+   - eauto.
+   - unfold assumes. destruct H0. 
+      * apply f in H0. left. names in H0. apply H0.
+      * destruct H0. apply f in H0. right. eauto. 
++ intros. names. apply aT_Sig with (x:=x). eauto.
+  names. apply IHpT2 with (Δ:= (Δ & x ~ Assum ([r] A0))) (r:= (r,, x)%ren).
+  apply ctx_rename; eauto. apply wf_Assum with (eUni (uType i)); eauto.
++  intros. names. apply aT_Pair with ([r] U).
+  - auto.
+  - specialize IHpT2 with (r:=r) (Δ:=Δ). names in IHpT2. apply IHpT2; eauto.
+  - specialize IHpT3 with (r:=r) (Δ:=Δ). names in IHpT3. apply IHpT3; eauto.
++  intros. names. eapply aT_Prod_Prop with (x:=x). eauto.
+  names. apply IHpT2 with (Δ:= (Δ & x ~ Assum ([r] A0))) (r:= (r,, x)%ren).
+  apply ctx_rename. auto. eauto.
++  intros. names. eapply aT_Prod_Type with (x:=x). eauto.
+  names. apply IHpT2 with (Δ:= (Δ & x ~ Assum ([r] A0))) (r:= (r,, x)%ren).
+  apply ctx_rename. auto. eauto.
++  intros. names. eapply aT_Lam with (x:=x). eauto.
+  names. apply IHpT2 with (Δ:= (Δ & x ~ Assum ([r] A0))) (r:= (r,, x)%ren).
+  apply ctx_rename. auto. apply wf_Assum with ([r] U); eauto.
++  intros. names. apply aT_Let with (x:=x) (A:=([r]A0)) (U:=([r]U)); eauto.
+  names. apply IHpT3 with (Δ:= (Δ & x ~ Def ([r] n) ([r] A0))) (r:= (r,, x)%ren).
+  apply ctx_rename. auto. apply wf_Def with ([r] U); eauto.
++  intros. names. apply aT_If with (x:=x) (p:=p) (U:=[r,,x]U). 
+  - names. apply IHpT1 with (Δ:= (Δ & x ~ Assum eBool)) (r:= (r,, x)%ren).
+    apply ctx_rename. auto. eauto.
+  - eauto.
+  - names. specialize IHpT3 with (Δ:= (Δ & p ~ Assum (eEqv ([r] e) eTru))) (r:= (r,, p)%ren). names in IHpT3. apply IHpT3.
+    apply ctx_rename. auto. eapply wf_Assum with (eUni (uType 0)). auto.
+    apply aT_Equiv with (B:= eBool); eauto.
+  - names. specialize IHpT4 with (Δ:= (Δ & p ~ Assum (eEqv ([r] e) eFls))) (r:= (r,, p)%ren). names in IHpT4. apply IHpT4.
+    apply ctx_rename. auto. eapply wf_Assum with (eUni (uType 0)). auto.
+    apply aT_Equiv with (B:= eBool); eauto.
++ intros. apply aT_Conv with (A:=[r]A0)(U:=[r]U); eauto.
+  apply SubTypes_weakening with g; auto.
++  intros. names. apply aT_App with ([r]A').
+  - apply IHpT1; auto.
+  - apply IHpT2; auto.
++ intros. names. apply aT_Fst with ([r]B). apply IHpT; auto.
++ intros. names. apply aT_Snd with ([r]A0). apply IHpT; auto.
++ intros. names. apply aT_Refl with ([r]A0). auto.
++ intros. names. apply aT_Equiv with (B:=[r]B); eauto.
+Qed.
 
-Definition WellFormed_weakening Γ (pWF: (⊢ Γ)):=
-  forall r Δ,
-    Γ =[r]=> Δ ->
-    (⊢ Δ).
-
-Theorem weakening {Γ e A pT pWF}:
+(* Theorem weakening {Γ e A pT pWF}:
 Type_weakening Γ e A pT /\ WellFormed_weakening Γ pWF.
 Proof.
 induction Types_WellFormed_mutind with (P:=Type_weakening) (P0:=WellFormed_weakening). auto.
-all: try (intros; constructor; eauto; fail); unfold Type_weakening.
-+ intros. names. destruct H0 eqn:H3. 
-  rewrite applyt_is_applyv with (rn:=total). names. apply aT_Var.
-   - eauto.
-   - unfold assumes. destruct a. 
-      * apply f in H1. left. names in H1. apply H1.
-      * destruct H1. apply f in H1. right. eauto.
-+ intros. names. apply aT_Sig with (x:=x). eauto.
-  names. apply H0 with (Δ:= (Δ & x ~ Assum ([r] A0))) (r:= (r,, x)%ren).
-  apply ctx_rename. auto.
-+  intros. names. apply aT_Pair.
-  - auto.
-  - specialize H0 with (r:=r) (Δ:=Δ). names in H0. apply H0. eauto.
-+  intros. names. eapply aT_Prod_Prop with (x:=x). eauto.
-  names. apply H0 with (Δ:= (Δ & x ~ Assum ([r] A0))) (r:= (r,, x)%ren).
-  apply ctx_rename. auto.
-+  intros. names. eapply aT_Prod_Type with (x:=x). eauto.
-  names. apply H0 with (Δ:= (Δ & x ~ Assum ([r] A0))) (r:= (r,, x)%ren).
-  apply ctx_rename. auto.
-+  intros. names. eapply aT_Lam with (x:=x). eauto.
-  names. apply H with (Δ:= (Δ & x ~ Assum ([r] A0))) (r:= (r,, x)%ren).
-  apply ctx_rename. auto.
-+  intros. names. eapply aT_Let with (x:=x). eauto.
-  names. apply H0 with (Δ:= (Δ & x ~ Def ([r] n) ([r] A0))) (r:= (r,, x)%ren).
-  apply ctx_rename. auto.
-+  intros. names. eapply aT_If with (x:=x). 
-  - names. apply H with (Δ:= (Δ & x ~ Assum eBool)) (r:= (r,, x)%ren).
-    apply ctx_rename. auto.
-  - eauto.
-  - names. specialize H1 with (Δ:= (Δ & p ~ Assum (eEqv ([r] e0) eTru))) (r:= (r,, p)%ren). names in H1. apply H1.
-    apply ctx_rename. auto.
-  - names. specialize H2 with (Δ:= (Δ & p ~ Assum (eEqv ([r] e0) eFls))) (r:= (r,, p)%ren). names in H2. apply H2.
-    apply ctx_rename. auto.
-+  intros. apply aT_Conv with (A:=[r]A0)(U:=[r]U); eauto.
-  apply SubTypes_weakening with g; auto.
-+  intros. names. apply aT_App with ([r]A').
-  - apply H. auto.
-  - apply H0. auto.
-+ intros. names. apply aT_Fst with ([r]B). apply H. auto.
-+ intros. names. apply aT_Snd with ([r]A0). apply H. auto.
-+ intros. names. apply aT_Refl with ([r]A0). auto.
-+ unfold WellFormed_weakening. intros.  
+all: try (intros; constructor; eauto; fail); unfold Type_weakening. *)
 
-
-Lemma weakening1 (g: env) (A U B: exp) (x: name):
-(g ⊢ A : U) ->
-(g & x ~ Assum B ⊢ [^x] A : U) /\ (forall e: exp, (g & x ~ Def e B ⊢ [^x] A : U)).
+Lemma cons_weakening_assum (g: env) (A A': exp) (x: name):
+(g ⊢ A : A') ->
+  (forall B B', 
+   ((g ⊢ B : B') -> 
+   (g & x ~ Assum B ⊢ [^x] A : [^x] A'))).
 Proof.
-Admitted.
+intros. apply Type_weakening with g; auto. apply ctx_shift; apply ctx_id.
+apply wf_Assum with B'; auto. apply Types_only_if_wellformed with A A'; auto. 
+Qed.
+
+Lemma cons_weakening_def (g: env) (A A': exp) (x: name):
+(g ⊢ A : A') ->
+  (forall B B' e, 
+   ((g ⊢ B : B') ->
+    (g ⊢ e : B) ->
+   (g & x ~ Def e B ⊢ [^x] A : [^x] A'))).
+Proof.
+intros. apply Type_weakening with g; auto. apply ctx_shift; apply ctx_id.
+apply wf_Def with B'; auto. apply Types_only_if_wellformed with A A'; auto.
+Qed.
 
 Require Import String.
 Open Scope string.
@@ -104,7 +136,7 @@ Proof. eapply wf_Def. apply WF_2.
   - apply aT_Ax_Prop. apply WF_2.
 Qed.
 
-Lemma typing_is_broken_part_1: 
+(* Lemma typing_is_broken_part_1: 
 ((ctx_empty & "x" ~ Def eBool (eUni (uType 0)) & "y" ~ Assum (eId (free "x"))) ⊢ eId (free "y") : eBool).
 Proof.
 eapply aT_Conv.
@@ -120,9 +152,9 @@ eapply aT_Conv.
 + apply ST_Cong. apply aE_Step with (e:=eBool).
   - apply R_RedR. apply st_ID with (A:= (eUni (uType 0))); auto with contexts.
   - apply R_Reflex.
-Qed.
+Qed. *)
 
-Lemma typing_is_broken_part_2: 
+(* Lemma typing_is_broken_part_2: 
 (((ctx_empty & "x" ~ Def eBool (eUni (uType 0))
             & "y" ~ Assum (eId (free "x")))
             & "x" ~ Def (eUni uProp) (eUni (uType 0))) ⊢ eId (free "y") : (eUni uProp)).
@@ -133,59 +165,94 @@ eapply aT_Conv.
 + apply ST_Cong. apply aE_Step with (e:=eUni uProp).
   - apply R_RedR. apply st_ID with (A:= (eUni (uType 0))). auto with contexts.
   - apply R_Reflex.
-Qed.
-
-
+Qed. *)
 (* Conclusion: We need to shift the bodies of ass/defs in the context when we add a new ass/def *)
 
-Lemma WellFormed_implies (g: env) (A: exp):
+
+Lemma WellFormed_implies_well_typed_assum (g: env):
 WellFormed g ->
-forall (x: name),
-assumes g (free x) A ->
-exists U, Types g ([^x]A) U.
+forall (v: var) (A: exp),
+(has g v (Assum A)) ->
+exists U, Types g A U.
 Proof.
-induction g. 
- - intros. inversion H0. inversion H1. inversion H1. inversion H2.
- - intros. inversion H. subst. inversion H0.
-   cbn in H1. destruct (closev a (free x)). Admitted.
-   
+induction 1.
++ intros. inversion H.
++ intros. rename H0 into H2. rename H1 into H0. rename H2 into H1. 
+  apply has_inversion in H0. apply get_inversion in H0.
+  destruct H0. destruct H0. inversion H0. subst.
+  destruct H2.
+  * destruct H0 as [g']. destruct H0 as [c]. destruct H0.
+    inversion H0. subst. names in H2. inversion H2. subst. destruct H0.
+    exists ([^x0] U). apply cons_weakening_assum with U; auto.
+  * destruct H0 as [g']. destruct H0. destruct H0 as [c]. destruct H0. destruct H0 as [c'].
+    destruct H0. destruct H2. destruct H3. inversion H0. subst. clear H0.
+    destruct H4. cut (has g' x2 c'). intro. cut (exists B, c' = Assum B). intro. 
+    destruct H5 as [B]. subst. names in H3. inversion H3. subst.
+    apply IHWellFormed in H4. destruct H4 as [B']. 
+    apply cons_weakening_assum with (A:=B) (A':=B')(x:=x1) in H1.
+    eauto. eauto. unfold apply in H3. destruct c'. eauto. discriminate.
+    unfold has. rewrite H0. auto.
++ intros. apply has_inversion in H2. apply get_inversion in H2.
+  destruct H2. destruct H2. destruct H3.
+  * destruct H3. destruct H3. destruct H3.
+    inversion H3. subst. inversion H4.
+  * destruct H3 as [g']. destruct H3. destruct H3 as [c]. destruct H3.
+    destruct H3 as [c']. destruct H3. destruct H4. destruct H5.
+    inversion H3. subst. clear H3.
+    cut (has g' x2 c'). cut (exists B, c' = Assum B). intros.
+    destruct H2 as [B]. subst. names in H6. inversion H6. subst.
+    apply IHWellFormed in H3. destruct H3 as [B'].
+    apply cons_weakening_def with (A:=B) (A':=B') (B':=U)(x:=x1) in H1.
+    all: eauto. unfold apply in H6. destruct c'. eauto. discriminate. unfold has. rewrite H5. auto.
+Qed.
 
-
-(* H1.
-  + cbn in H1. destruct (bindv (closev x (free x0))).
-    * cut (assumes g v A).
-      -- intros. cut (exists n, v = free n).
-         ** intros. destruct H3. subst. apply IHWellFormed in H2. destruct H2. exists x2. apply weakening1. auto. 
-      -- auto.
-    * inversion H1. subst. exists U. apply weakening1. auto.
-  + cbn in H1. destruct (bindv (closev x x0)).
-    * cut (assumes g v A).
-      -- intros. apply IHWellFormed in H2. destruct H2. exists x1. apply weakening1. auto. 
-      -- auto.
-    * inversion H1. inversion H2.
-  - intros. destruct H2.
-    + cbn in H2. destruct (bindv (closev x x0)).
-      * cut (assumes g v A).
-        -- intros. apply IHWellFormed in H3. destruct H3. exists x1. apply weakening1. auto. 
-        -- auto.
-      * inversion H2.
-    + cbn in H2. destruct (bindv (closev x x0)).
-      * cut (assumes g v A).
-        -- intros. apply IHWellFormed in H3. destruct H3. exists x1. apply weakening1. auto. 
-        -- auto.
-      * inversion H2. inversion H3. subst. exists U. apply weakening1. auto.
-Qed. *)
-
-
+Lemma WellFormed_implies_well_typed_def (g: env):
+WellFormed g ->
+forall (v: var) (A: exp) (e: exp),
+(has g v (Def e A)) ->
+exists U, Types g A U.
+Proof.
+induction 1.
++ intros. inversion H.
++ intros. rename H0 into H2. rename H1 into H0. rename H2 into H1. 
+  apply has_inversion in H0. apply get_inversion in H0.
+  destruct H0. destruct H0. inversion H0. subst.
+  destruct H2.
+  * destruct H0. destruct H0. destruct H0. inversion H0. subst. inversion H2. 
+  * destruct H0 as [g']. destruct H0. destruct H0 as [c]. destruct H0. destruct H0 as [c'].
+    destruct H0. destruct H2. destruct H3. inversion H0. subst. clear H0.
+    destruct H4. cut (has g' x2 c'). intro. cut (exists e' B, c' = Def e' B). intro. 
+    destruct H5 as [e']. destruct H5 as [B]. subst. names in H3. inversion H3. subst.
+    apply IHWellFormed in H4. destruct H4 as [B']. 
+    apply cons_weakening_assum with (A:=B) (A':=B')(x:=x1) in H1.
+    eauto. eauto. unfold apply in H3. destruct c'. discriminate. eauto.
+    unfold has. rewrite H0. auto.
++ intros. apply has_inversion in H2. apply get_inversion in H2.
+  destruct H2. destruct H2. destruct H3.
+  * destruct H3 as [g']. destruct H3 as [c]. destruct H3.
+    inversion H3. subst. names in H4. inversion H4. subst. destruct H4.
+    exists ([^x0] U). apply cons_weakening_def with U; auto.
+  * destruct H3 as [g']. destruct H3. destruct H3 as [c]. destruct H3. destruct H3 as [c'].
+    destruct H3. destruct H4. destruct H5. inversion H3. subst. clear H3.
+    cut (has g' x2 c'). intro. cut (exists e' B, c' = Def e' B). intro. 
+    destruct H3 as [e']. destruct H3 as [B]. subst. names in H6. inversion H6. subst.
+    apply IHWellFormed in H2. destruct H2 as [B']. exists ([^x1] B').
+    apply cons_weakening_def with (A:=B) (A':=B')(x:=x1) (B':=U); eauto.
+    unfold apply in H6. destruct c'. discriminate. eauto.
+    unfold has. rewrite H5. auto.
+Qed.
 
 Lemma type_well_typed (g: env) (N: exp) (A: exp) :
   (g ⊢ N : A) ->
-  exists U , Types g A U.
+  exists U , Types g A (eUni (uType i)).
 Proof.
-  induction 1.
-  - exists (eUni (uType 1)). apply aT_Ax_Type. auto.
-  - exists (eUni (uType (S (S i)))). apply aT_Ax_Type. auto.
-  - intros. Admitted. (*  apply WellFormed_implies. intros. induction H0.
+  induction 1; eauto.
+  - intros. destruct H0.
+    + apply WellFormed_implies_well_typed_assum with (v:=x); auto.
+    + destruct H0 as [e]. apply WellFormed_implies_well_typed_def with (v:=x) (e:=e); auto.
+  -  
+  
+  Admitted. (*  apply WellFormed_implies. intros. induction H0.
     + subst. destruct H; destruct h. 
     + subst. destruct H. cbn in h. destruct (bindv (closev x0 x)).
       * names.  
